dynamic_dependent_tactic.v
@@ -32,11 +32,11 @@ Section insert.
       tree s1 o1 d cl -> tree s2 o2 d cr ->
       tree (s1 + s2) (o1 + o2) (incr_black d c) c.*)
 
-  Fixpoint size_of_tree {s o d c} (t : tree w s o d c) : nat :=
+(*  Fixpoint size_of_tree {s o d c} (t : tree w s o d c) : nat :=
     match t with
     | Leaf _ _ s => 1
     | Node _ _ _ _ _ _ _ _ _ _ l r => size_of_tree l + size_of_tree r
-    end.
+    end.*)
 
   Lemma size_of_tree_pos num ones d c (B : tree w num ones d c) :
     size_of_tree B > 0.
